Proved correctness of inference steps.

checker/coq/log.v
@@ -22,9 +22,9 @@ Definition state := ((zmap cst) * (zmap clause) * Z)%type.
 
 Ltac destate s := destruct s as (p, h) ; destruct p as (cs, cls).
 Inductive status :=
-  | Valid
-  | Invalid
-  | Incomplete : state -> status.
+  | Unknown
+  | Unsat
+  | Invalid : step -> status.
 
 Definition eval_cstmap cs theta :=
   forall (id : Z) (c : cst),
@@ -34,6 +34,9 @@ Definition state_csts (s : state) :=
   match s with
   | (cs, clauses, hint) => cs
   end.
+
+Definition eval_clauses (cs : list clause) theta :=
+  forall cl, List.In cl cs -> eval_clause cl theta.
 
 Definition eval_clmap clauses theta :=
   forall id cl, ZMaps.MapsTo id cl clauses -> eval_clause cl theta.
@@ -54,7 +57,6 @@ Definition state_valid (s : state) :=
 Definition clause_map_add (cs : clause_map) (id : Z) (cl : clause) := ZMaps.add id cl cs.
 
 Definition clause_map_del (cs : clause_map) (id : Z) := ZMaps.remove id cs.
-
 
 Lemma clause_map_1 : forall cs cl id theta,
   eval_clmap cs theta -> eval_clause cl theta -> eval_clmap (clause_map_add cs id cl) theta.
@@ -81,17 +83,24 @@ Definition check_inference (s : state) (cl : clause) :=
     end
   end.
 
-(*
-Lemma check_inference_valid : forall (s : state) (cl : clause) (theta : asg),
-  check_inference s cl = true -> eval_cstmap (state_csts s) theta -> eval_clause cl theta.
+Lemma check_inference_valid_2 : forall (s : state) (cl : clause),
+  check_inference s cl = true -> forall theta, eval_cstmap (state_csts s) theta -> eval_clause cl theta.
 Proof.
-  (* Add proof *)
+  unfold check_inference; destate s; unfold eval_cstmap; intros.
+  remember (ZMaps.find h cs) as fh; destruct fh; simpl in *.
+    symmetry in Heqfh; apply find_mapsto_iff in Heqfh.
+    apply check_cst_valid with (c := c). assumption. now apply H0 with (id := h).
+    discriminate.
 Qed.
-*)
 
-Definition apply_inference (s : state) (id : Z) (cl : clause) := Invalid.
-Definition apply_resolution (s : state) (id : Z) (cl : clause) (ants : list Z) := Invalid.
-
+Lemma check_inference_valid : forall (s : state) (cl : clause),
+   check_inference s cl = true -> inference_valid s cl.
+Proof.
+  intros.
+  unfold inference_valid; intros; destate s; intros.
+  now apply check_inference_valid_2 with (s := ((cs, cls), h)) (theta := theta).
+Qed.
+  
 Definition set_hint (s : state) (hint : Z) : state:=
   match s with
   | (csts, clauses, old) => (csts, clauses, hint)
@@ -129,17 +138,84 @@ Proof.
   destruct Hdis as [Hid Hmap].
   now  apply H with (id := id0) (cl := cl0) (theta := theta).
 Qed.
-  
-Definition apply_step (s : status) (d : step) :=
-  match s with
-  | Valid => Valid
-  | Invalid => Invalid
-  | Incomplete state =>
-    match d with
-    | Intro cid cl => apply_inference state cid cl
-    | Hint cid => Incomplete (set_hint state cid)
-    | Del cid => Incomplete (del_clause state cid)
-    | Resolve cid cl ants => apply_resolution state cid cl ants
-    end
+
+Definition apply_inference (s : state) (id : Z) (cl : clause) :=
+  if check_inference s cl then
+    add_clause s id cl
+  else
+    s.
+Lemma apply_inference_valid : forall s id cl,
+  state_valid s -> state_valid (apply_inference s id cl).
+Proof.
+  unfold apply_inference; simpl; intros.
+  remember (check_inference s cl) as c; symmetry in Heqc; destruct c.
+  apply add_clause_valid.
+    assumption.
+    now apply check_inference_valid. assumption.
+Qed.
+
+
+ 
+Fixpoint clauses_deref (cs : clause_map) (ids : list Z) :=
+  match ids with
+  | nil => nil
+  | cons id ids' =>
+      let rest := clauses_deref cs ids' in
+      match ZMaps.find id cs with
+      | None => rest
+      | Some cl => cons cl rest
+      end
   end.
-    
+
+  
+Theorem clauses_deref_1 : forall cs ids theta,
+  eval_clmap cs theta -> eval_clauses (clauses_deref cs ids) theta.
+Proof.
+  unfold eval_clmap, eval_clauses; intros; induction ids.
+  unfold clauses_deref in *; now apply List.in_nil in H0.
+  unfold clauses_deref in H0; fold clauses_deref in H0.
+  remember (ZMaps.find a cs) as fa.
+  destruct fa; simpl in *.
+  destruct H0 as [Heq | Hin] ;
+    [rewrite <- Heq; symmetry in Heqfa; apply H with (id := a); now apply find_mapsto_iff | apply IHids ; now apply Hin].
+  now apply IHids.
+Qed.
+
+Definition get_clauses (s : state) (ids : list Z) :=
+  match s with
+  | (cs, cls, h) => clauses_deref cls ids
+  end.
+
+Definition apply_resolution (s : state) (id : Z) (cl : clause) (ants : list Z) :=
+  if resolvable cl (get_clauses s ants) then
+    add_clause s id cl
+  else
+    s.
+Lemma apply_resolution_valid : forall (s : state) (id : Z) (cl : clause) (ants : list Z),
+  state_valid s -> state_valid (apply_resolution s id cl ants).
+Proof.
+  intros; unfold apply_resolution.
+  remember (resolvable cl (get_clauses s ants)) as r; symmetry in Heqr; destruct r; simpl in *;
+    try assumption.
+  remember (get_clauses s ants) as acl.
+  apply add_clause_valid; try assumption.
+  unfold inference_valid; destate s; intros.
+  now apply resolvable_valid with (theta := theta) (ants := acl).
+Qed.
+
+Definition apply_step (s : state) (d : step) :=
+  match d with
+  | Intro cid cl => apply_inference s cid cl
+  | Hint cid => set_hint s cid
+  | Del cid => del_clause s cid
+  | Resolve cid cl ants => apply_resolution s cid cl ants
+   end.
+Theorem apply_step_valid : forall (s : state) (d : step),
+  state_valid s -> state_valid (apply_step s d).
+Proof.
+  intros; unfold apply_step; destruct d; simpl in *.
+    now apply apply_inference_valid.
+    now apply set_hint_valid.
+    now apply del_clause_valid.
+    now apply apply_resolution_valid.
+Qed.
